theories/extraction.v
@@ -2,8 +2,22 @@ From Stdlib Require Import Extraction.
 From Stdlib Require Import ExtrOcamlBasic.
 From Stdlib Require Import ExtrOcamlString.
 From Stdlib Require Import ExtrOcamlNatInt.
+From Stdlib Require Import Strings.String.
 
-From wasmcomponents Require Import wit_ast wit_parser.
+From wasmcomponents Require Import wit_ast component_ast component_binary_parser wit_parser.
 
 Set Extraction Output Directory "src/extraction".
-Separate Extraction parse_wit.
+
+Definition parse_component_ok (s : string) : bool :=
+  match run_parse_component_str s with
+  | inl _ => true
+  | inr _ => false
+  end.
+
+Definition parse_component_error (s : string) : option string :=
+  match run_parse_component_str s with
+  | inl _ => None
+  | inr e => Some e
+  end.
+
+Separate Extraction parse_wit parse_component_ok parse_component_error.
